\documentclass[12pt]{article}
 
\usepackage[margin=1in]{geometry} 
\usepackage{amsmath,amsthm,amssymb,scrextend}
\usepackage{fancyhdr}
\setlength{\headheight}{14.5pt}
\addtolength{\topmargin}{-2.5pt}
\pagestyle{fancy}

\newcommand{\cont}{\subseteq}
\usepackage{tikz}
\usepackage{pgfplots}
\usepackage{amsmath}
\usepackage[mathscr]{euscript}
\let\euscr\mathscr\let\mathscr\relax% just so we can load this and rsfs
\usepackage[scr]{rsfso}
\usepackage{amsthm}
\usepackage{amssymb}
\usepackage{multicol}
\usepackage[colorlinks=true, pdfstartview=FitV, linkcolor=blue,
citecolor=blue, urlcolor=blue]{hyperref}

\DeclareMathOperator{\arcsec}{arcsec}
\DeclareMathOperator{\arccot}{arccot}
\DeclareMathOperator{\arccsc}{arccsc}
\newcommand{\ddx}{\frac{d}{dx}}
\newcommand{\dfdx}{\frac{df}{dx}}
\newcommand{\ddxp}[1]{\frac{d}{dx}\left(#1 \right)}
\newcommand{\dydx}{\frac{dy}{dx}}
\let\ds\displaystyle
\newcommand{\intx}[1]{\int#1 \, dx}
\newcommand{\intt}[1]{\int#1 \, dt}
\newcommand{\defint}[3]{\int_{#1}^{#2} #3 \, dx}
\newcommand{\imp}{\Rightarrow}
\newcommand{\un}{\cup}
\newcommand{\inter}{\cap}
\newcommand{\ps}{\mathscr{P}}
\newcommand{\set}[1]{\left\{ #1 \right\}}
\newtheorem*{sol}{Solution}
\newtheorem*{claim}{Claim}
\newtheorem{problem}{Problem}
\pgfplotsset{compat=1.17}
\begin{document}
 
% Don't change the above session

\lhead{Financial Engineering hw3}
\chead{111352027}
\rhead{\today}
 
% \maketitle
\section*{Fourier Transformation I}
Proof $-i\lambda F(\lambda)$ is $f'(x)$'s Fourier Transformation\\\\
Given $F(\lambda) = F_x[f(x)](\lambda) = \int_{-\infty}^{\infty} e^{i\lambda x} f(x) \, dx$
\newline
\begin{align*}
    F_x[f'(x)](\lambda) & = \int_{-\infty}^{\infty} e^{i\lambda x} f'(x) \, dx \\
\end{align*}
According to integral by parts\\
\[
    \int u \, dv = uv - \int v \, du
\]  
\newline
Let $dv = f'(x)dx$, $u = e^{i\lambda x}$. So $v = f(x)$, $du = i\lambda e^{i\lambda x}\, dx$\\
\begin{align*}
    F_x[f'(x)](\lambda) & = f(x)e^{i \lambda x}\Big]_{-\infty}^{\infty} - \int_{-\infty}^{\infty}f(x)(i\lambda e^{i \lambda x})\,  dx\\
\end{align*}
Because $\lim_{x\to\pm\infty}f(x)=0$\\
\begin{align*}
    F_x[f'(x)](\lambda) = -i\lambda \int_{-\infty}^{\infty}f(x)e^{i \lambda x}\, dx = -i\lambda F(\lambda)
\end{align*}
\section*{Fourier Transformation II}
Proof $(-i\lambda)^n F(\lambda)$ is $f^{(n)}(x)$'s Fourier Transformation\\\\
Given $F(\lambda) = F_x[f(x)](\lambda) = \int_{-\infty}^{\infty} e^{i\lambda x} f(x) \, dx$
\newline
\begin{align*}
    F_x[f^{(n)}(x)](\lambda) & = \int_{-\infty}^{\infty} e^{i\lambda x} f^{(n)}(x) \, dx \\
\end{align*}
According to integral by parts\\
\[
    \int u \, dv = uv - \int v \, du
\]
\newline
Let $dv = f^{(n)}(x)dx$, $u = e^{i\lambda x}$. So $v = f^{(n-1)}(x)$, $du = i\lambda e^{i\lambda x}\, dx$\\
\begin{align*}
    F_x[f^{(n)}(x)](\lambda) & = f^{(n-1)}(x)e^{i \lambda x}\Big]_{-\infty}^{\infty} - \int_{-\infty}^{\infty}f^{(n-1)}(x)(i\lambda e^{i \lambda x})\,  dx\\
\end{align*}
Because $\lim_{x\to\pm\infty}f^{(n-1)}(x)=0$\\
\begin{align*}
    F_x[f^{(n)}(x)](\lambda) & = -i\lambda \int_{-\infty}^{\infty}f^{(n-1)}(x)e^{i \lambda x}\, dx = -i\lambda F_x[f^{(n-1)}(x)](\lambda)\\\\
    & = (-i\lambda)^2 F_x[f^{(n-2)}(x)](\lambda)\\\\
    & = \cdots = (-i\lambda)^n F_x[f(x)](\lambda) = (-i\lambda)^n F(\lambda) 
\end{align*}
\section*{Fourier Inverse Transformation I}
Given $F(\lambda) = e^{i\mu\lambda+\frac{i^2\lambda^2\sigma^2}{2}}$, get $f(x)$ by Fourier Inverse Transformation\\\\
\begin{align*}
    f(x) & = \int_{-\infty}^{\infty} \dfrac{1}{2\pi}e^{-i\lambda x}F(\lambda)d\lambda\\
    & = \dfrac{1}{2\pi}\int_{-\infty}^{\infty} e^{i\lambda x}e^{i\mu\lambda+\frac{i^2\lambda^2\sigma^2}{2}}d\lambda\\
    & = \dfrac{1}{2\pi}\int_{-\infty}^{\infty} e^{i\lambda(\mu-x)+\frac{i^2\lambda^2\sigma^2}{2}}d\lambda\\
    & = \dfrac{1}{2\pi}\times \Bigg[\dfrac{1}{i(\mu-x)+i^2\sigma^2\lambda}e^{i\lambda(\mu-x)+\frac{i^2\lambda^2\sigma^2}{2}}\Bigg]_{-\infty}^{\infty}\\
    & = \dfrac{1}{2\pi}\times[0-0]=0
\end{align*}
\end{document}